
\begin{align}
H_{E} = \frac{g^{2} \left(4 \sum_{\nu=1}^{16} \frac{fc_{\nu} \left(U_{10y}^{\nu} + U_{10yD}^{\nu}\right)}{2} + 4 \sum_{\nu=1}^{16} \frac{fc_{\nu} \left(U_{11y}^{\nu} + U_{11yD}^{\nu}\right)}{2} + 6 \sum_{\nu=1}^{16} \frac{fc_{\nu} \left(U_{20y}^{\nu} + U_{20yD}^{\nu}\right)}{2} + 6 \sum_{\nu=1}^{16} \frac{fc_{\nu} \left(U_{21y}^{\nu} + U_{21yD}^{\nu}\right)}{2} - 2 \left(\sum_{\nu=1}^{16} - 0.5 i fs_{\nu} \left(U_{10y}^{\nu} - U_{10yD}^{\nu}\right)\right) \sum_{\nu=1}^{16} - 0.5 i fs_{\nu} \left(U_{11y}^{\nu} - U_{11yD}^{\nu}\right) + 6 \left(\sum_{\nu=1}^{16} - 0.5 i fs_{\nu} \left(U_{10y}^{\nu} - U_{10yD}^{\nu}\right)\right) \sum_{\nu=1}^{16} - 0.5 i fs_{\nu} \left(U_{20y}^{\nu} - U_{20yD}^{\nu}\right) - 2 \left(\sum_{\nu=1}^{16} - 0.5 i fs_{\nu} \left(U_{10y}^{\nu} - U_{10yD}^{\nu}\right)\right) \sum_{\nu=1}^{16} - 0.5 i fs_{\nu} \left(U_{21y}^{\nu} - U_{21yD}^{\nu}\right) + 2 \sum_{\nu=1}^{16} - 0.5 i fs_{\nu} \left(U_{10y}^{\nu} - U_{10yD}^{\nu}\right) - 2 \left(\sum_{\nu=1}^{16} - 0.5 i fs_{\nu} \left(U_{11y}^{\nu} - U_{11yD}^{\nu}\right)\right) \sum_{\nu=1}^{16} - 0.5 i fs_{\nu} \left(U_{20y}^{\nu} - U_{20yD}^{\nu}\right) + 6 \left(\sum_{\nu=1}^{16} - 0.5 i fs_{\nu} \left(U_{11y}^{\nu} - U_{11yD}^{\nu}\right)\right) \sum_{\nu=1}^{16} - 0.5 i fs_{\nu} \left(U_{21y}^{\nu} - U_{21yD}^{\nu}\right) + 4 \sum_{\nu=1}^{16} - 0.5 i fs_{\nu} \left(U_{11y}^{\nu} - U_{11yD}^{\nu}\right) - 4 \left(\sum_{\nu=1}^{16} - 0.5 i fs_{\nu} \left(U_{20y}^{\nu} - U_{20yD}^{\nu}\right)\right) \sum_{\nu=1}^{16} - 0.5 i fs_{\nu} \left(U_{21y}^{\nu} - U_{21yD}^{\nu}\right) + 2 \sum_{\nu=1}^{16} - 0.5 i fs_{\nu} \left(U_{20y}^{\nu} - U_{20yD}^{\nu}\right) + 4 \sum_{\nu=1}^{16} - 0.5 i fs_{\nu} \left(U_{21y}^{\nu} - U_{21yD}^{\nu}\right) + 3\right)}{2}\\
H_{B} = - \frac{\cos{\left(E_{10y} α \right)} + \cos{\left(E_{11y} α \right)} + \cos{\left(α \left(- E_{10y} + E_{20y}\right) \right)} + \cos{\left(α \left(- E_{11y} + E_{21y}\right) \right)}}{g^{2}}
\end{align}
